Splinter/CacheLemmas.i.dfy
@@ -4,7 +4,7 @@ module CacheLemmasMod {
   import opened CacheIfc
 
   lemma EquivalentCaches(cache: Variables, cache': Variables, cacheOps: Ops)
-    requires ApplyWrites(cache, cache', cacheOps)
+    requires WritesApplied(cache, cache', cacheOps)
     requires cacheOps == []
     ensures cache.dv == cache'.dv
   {
