Splinter/JournalInterp.i.dfy
@@ -25,61 +25,11 @@ module JournalInterpMod {
   predicate Invariant(v: Variables, cache: CacheIfc.Variables)
   {
     && v.WF()
-    && var optChain := ChainFrom(cache.dv, v.CurrentSuperblock()).chain;
-    && optChain.Some?
-    && ValidJournalChain(cache.dv, optChain.value)
-    // Superblocks says chain ends where variables says it should
-    && v.marshalledLSN == (
-        if |optChain.value.recs|==0
-        then v.boundaryLSN
-        else optChain.value.recs[0].messageSeq.seqEnd
-      )
+    && v.marshalledLookup.ValidForSB(cache, v.CurrentSuperblock())
+    && v.marshalledLookup.last().expectedEnd.None?  // consider rolling this into ValidForSB, which isn't used inductively -- I think?
   }
 
-  // Interpret the chain of marshalled LSNs plus the unmarshalledTail as a MsgSeq
-  function ChainAsMsgSeq(v: Variables, cache:CacheIfc.Variables) : (result : MsgSeq)
-    requires v.WF()
-    requires Invariant(v, cache)
-    ensures result.WF()
-    ensures result.IsEmpty() ==> v.boundaryLSN == v.unmarshalledLSN()
-    ensures !result.IsEmpty() ==> result.seqEnd == v.unmarshalledLSN()
-    ensures !result.IsEmpty() ==> v.boundaryLSN == result.seqStart
-  {
-    // chain has all the marshalled messages
-    var chain := ChainFrom(cache.dv, v.CurrentSuperblock()).chain.value;
-
-    // tail has all the unmarshalled messages
-    var tailMsgs := TailToMsgSeq(v);
-
-    // we need to return all the messages in the journal. So let's join them together
-    assert !chain.interp.IsEmpty() && !tailMsgs.IsEmpty() ==>
-      chain.interp.seqEnd == tailMsgs.seqStart by {
-      if !chain.interp.IsEmpty() && !tailMsgs.IsEmpty() {
-        calc {
-          chain.interp.seqEnd;
-          chain.recs[0].messageSeq.seqEnd;
-          v.marshalledLSN;
-          tailMsgs.seqStart;
-        }
-      }
-    }
-    var result := chain.interp.Concat(tailMsgs);
-    assert !chain.interp.IsEmpty() ==> v.boundaryLSN == chain.interp.seqStart;
-    assert chain.interp.IsEmpty() && !tailMsgs.IsEmpty()
-      ==> v.boundaryLSN == tailMsgs.seqStart by {
-      if (chain.interp.IsEmpty() && !tailMsgs.IsEmpty()) {
-        calc {
-          v.boundaryLSN;
-//          sb.boundaryLSN;
-          tailMsgs.seqStart;
-        }
-      }
-    }
-//    assert chain.interp.IsEmpty() && tailMsgs.IsEmpty()
-//      ==> v.boundaryLSN == tailMsgs.seqStart;
-    assert !result.IsEmpty() ==> result.seqEnd == v.unmarshalledLSN();
-    result
-  }
+  // XXX was ChainAsMsgSeq now v.marshalledLookup.interp
 
   function SyncReqsAt(v: Variables, lsn: LSN) : set<CrashTolerantMapSpecMod.SyncReqId>
     //requires v.persistentLSN <= lsn < v.unmarshalledLSN()
@@ -89,18 +39,19 @@ module JournalInterpMod {
     set lsns |  v.persistentLSN <= lsns <= lsn
   }
 
+  function UnmarshalledMessageSeq(v: Variables, cache:CacheIfc.Variables) : MsgSeq
+    requires v.WF()
+  {
+    v.marshalledLookup.interp().Concat(TailToMsgSeq(v))
+  }
+
   function InterpFor(v: Variables, cache:CacheIfc.Variables, base: InterpMod.Interp, lsn: LSN) : Interp
     requires v.WF()
     requires Invariant(v, cache)
     requires base.seqEnd == v.boundaryLSN
     requires v.boundaryLSN <= lsn < v.unmarshalledLSN()
   {
-    var newMsqSeq := ChainAsMsgSeq(v, cache);
-    assert newMsqSeq.seqStart <= lsn < newMsqSeq.seqEnd;
-
-    var trucatedSeq := newMsqSeq.Truncate(lsn);
-    var interp := trucatedSeq.ApplyToInterp(base);
-    interp
+    UnmarshalledMessageSeq(v, cache).Truncate(lsn).ApplyToInterp(base)
   }
 
    function VersionFor(v: Variables, cache:CacheIfc.Variables, base: InterpMod.Interp, lsn: LSN) : CrashTolerantMapSpecMod.Version
@@ -135,7 +86,8 @@ module JournalInterpMod {
   function IMNotRunning(cache: CacheIfc.Variables, sb: Superblock, base: InterpMod.Interp) : CrashTolerantMapSpecMod.Variables
     requires base.seqEnd == sb.boundaryLSN  // This crash-invariant condition should probably not be a requires; just return nonsense if it fails.
   {
-    var pretendVariables := Variables(sb.boundaryLSN, sb.boundaryLSN, sb.boundaryLSN, sb.boundaryLSN, [], map[], map[]);
+    assume false; // this is all nonsense
+    var pretendVariables := Variables(sb.boundaryLSN, sb.boundaryLSN, sb.boundaryLSN, sb.boundaryLSN, [], map[], EmptyChainLookup(Superblock(None, 0), None));
     var versions := Versions(pretendVariables, cache, base);
     CrashTolerantMapSpecMod.Variables(versions, 0) // TODO Sowmya pick up here
   }
@@ -155,64 +107,53 @@ module JournalInterpMod {
   // repr-state style (see ReprsAsSets.i.dfy).
   function IReads(cache:CacheIfc.Variables, sb: Superblock) : seq<CU>
   {
-    ChainFrom(cache.dv, sb).readCUs
+    ChainFrom(cache, sb).last().cumulativeReadCUs
   }
 
-  lemma DiskViewsEquivalentAfterRemove(cache0: CacheIfc.Variables, cache1: CacheIfc.Variables, cus: seq<CU>, removedCU: CU, cusr: seq<CU>)
-    requires DiskViewsEquivalentForSeq(cache0.dv, cache1.dv, cus)
-    requires SequenceSubset(cusr, cus)
-    ensures DiskViewsEquivalentForSeq(MapRemove1(cache0.dv, removedCU), MapRemove1(cache1.dv, removedCU), cusr)
+  lemma CuInIReads(cl: ChainLookup, idx: nat)
+    requires 0 <= idx < |cl.rows|
+    requires cl.rows[idx].sb.freshestCU.Some?
+    ensures cl.rows[idx].sb.freshestCU.value in cl.last().cumulativeReadCUs
   {
   }
-
-  // TODO(jonh): delete chain parameter.
-  lemma FrameOneChain(cache0: CacheIfc.Variables, cache1: CacheIfc.Variables, sb: Superblock)
-    requires DiskViewsEquivalentForSeq(cache0.dv, cache1.dv, IReads(cache0, sb))
-    ensures ChainFrom(cache0.dv, sb) == ChainFrom(cache1.dv, sb)
-    decreases |cache0.dv|
+  
+  // This lemma dominates UniqueChainLookup.
+  lemma FrameOneChainInductive(cache0: CacheIfc.Variables, cache1: CacheIfc.Variables, sb: Superblock, cl0: ChainLookup, cl1: ChainLookup)
+    requires cl0.ValidForSB(cache0, sb)
+    requires cl1.ValidForSB(cache1, sb)
+    requires DiskViewsEquivalentForSeq(cache0.dv, cache1.dv, cl0.last().cumulativeReadCUs)
+    requires cl0.last().expectedEnd == cl1.last().expectedEnd
+    ensures cl0 == cl1
+    decreases |cl0.rows|
   {
+    assert cl0.Linked(|cl0.rows|-1);  // trigger
+    assert cl0.Linked(|cl0.rows|-1);  // trigger
+
     if sb.freshestCU.Some? {
-      assert sb.freshestCU.value in IReads(cache1, sb); // trigger
-      assert sb.freshestCU.value in IReads(cache0, sb); // trigger
-      assert IReads(cache0, sb)[0] == sb.freshestCU.value; // trigger
-      if sb.freshestCU.value in cache0.dv {
-        var firstRec := parse(cache0.dv[sb.freshestCU.value]);
-        if firstRec.Some? { // Recurse to follow chain
-          if firstRec.value.messageSeq.seqEnd <= sb.boundaryLSN {
-          } else if firstRec.value.messageSeq.seqStart <= sb.boundaryLSN  {
-          } else {
-            // TODO wrapping these back up in CacheIfcs seems clumsy. (and demands the stupid decreases clause)
-            var cache0r := CacheIfc.Variables(MapRemove1(cache0.dv, sb.freshestCU.value));
-            var cache1r := CacheIfc.Variables(MapRemove1(cache1.dv, sb.freshestCU.value));
-            var priorCU := firstRec.value.priorCU;
-            var priorSB := firstRec.value.priorSB(sb);
-            var cus := IReads(cache0, sb);
-            var cusr := if priorCU.Some?
-              then IReads(cache0r, priorSB)
-              else [];
+      assert sb.freshestCU.value in cl0.last().cumulativeReadCUs; // observe trigger
+    }
+    assert cl1.Linked(|cl1.rows| - 1);  // observe trigger -- lets us conclude cl1 has ==1 or >1 rows based on FirstRow() properties.
 
-            forall i | 0<=i<|cusr| ensures cusr[i] in cus {
-              assert cus[i+1] == cusr[i]; // witness to SequenceSubset(ausr, aus)
-            }
-            DiskViewsEquivalentAfterRemove(cache0, cache1, cus, sb.freshestCU.value, cusr);
-            FrameOneChain(cache0r, cache1r, priorSB);
-          }
-        }
-      }
+    if 1 < |cl0.rows| {
+      ValidPrior(cache0, cl0);
+      assert sb.freshestCU.value in cl0.last().cumulativeReadCUs; // observe trigger
+      ValidPrior(cache1, cl1);
+      var priorSB := cl0.rows[|cl0.rows|-2].sb;
+      assert cl1.DropLast().ValidForSB(cache1, priorSB);  // trigger
+
+//      assert cl0.DropLast().last().cumulativeReadCUs <= cl0.last().cumulativeReadCUs; // observe trigger
+      FrameOneChainInductive(cache0, cache1, priorSB, cl0.DropLast(), cl1.DropLast()); // recurse
     }
   }
 
-  lemma MappingLemma(v: Variables, cache: CacheIfc.Variables, newCU: CU, sb: Superblock, cr: ChainResult)
-    requires v.WF()
-    requires sb == Superblock(Some(newCU), v.boundaryLSN)
-    requires cr == ChainFrom(cache.dv, sb)
-    requires v.lsnToCU == MappingFor(cache, sb)
-    requires parse(ReadValue(cache, newCU)) == Some(JournalRecord(TailToMsgSeq(v), priorCU);
-    ensures cr.chain.Some?
-    ensures CUForChainIdx(cr.chain.value, 0) == newCU
+  lemma FrameOneChain(cache0: CacheIfc.Variables, cache1: CacheIfc.Variables, sb: Superblock)
+    requires DiskViewsEquivalentForSeq(cache0.dv, cache1.dv, IReads(cache0, sb))
+    ensures ChainFrom(cache0, sb) == ChainFrom(cache1, sb)
   {
-      //assert ChainFrom(cache.dv, sb).readCUs[0] == newCU
-    reveal_MappingFor();
+    var cl0 := ChainFrom(cache0, sb);
+    var cl1 := ChainFrom(cache1, sb);
+    FrameOneChainInductive(cache0, cache1, sb, cl0, cl1);
+    UniqueChainLookup(cache0, cl0, cl1);
   }
 
   // Add comment about what this supposed to do the TODOS here
@@ -224,7 +165,7 @@ module JournalInterpMod {
     requires Invariant(v', cache')
     requires v.boundaryLSN < v.unmarshalledLSN()
     requires Internal(v, v', cache, cacheOps, sk);
-    requires CacheIfc.ApplyWrites(cache, cache', cacheOps)
+    requires CacheIfc.WritesApplied(cache, cache', cacheOps)
     ensures v.boundaryLSN == v'.boundaryLSN
     ensures v.unmarshalledLSN() == v'.unmarshalledLSN()
     ensures IM(v, cache, base) == IM(v', cache', base)
@@ -236,86 +177,98 @@ module JournalInterpMod {
     {
       match sk {
         case AdvanceMarshalledStep(newCU) => {
-          assert ChainFrom(cache'.dv, v'.CurrentSuperblock()).chain.Some?;
-          var sb := v.CurrentSuperblock();
-          var sb' := v'.CurrentSuperblock();
-          var orig_chain_msgseq := ChainFrom(cache.dv, sb).chain.value.interp;
-          var orig_tail_msgseq := TailToMsgSeq(v);
-          var new_chain_msgseq := ChainFrom(cache'.dv, sb').chain.value.interp;
-          var new_tail_msgseq := TailToMsgSeq(v');
-
-          var priorCU := if v.marshalledLSN == v.boundaryLSN then None else Some(v.lsnToCU[v.marshalledLSN-1]);
-          var jr := JournalRecord(TailToMsgSeq(v), priorCU);
-          var sb_old := jr.priorSB(sb');
-          assert sb_old == sb;
-
-          assert newCU !in IReads(cache, sb);
-          assert DiskViewsEquivalentForSeq(cache.dv, cache'.dv, IReads(cache, sb));
-          FrameOneChain(cache, cache', sb);
-//          assert ChainFrom(cache.dv, sb).chain == ChainFrom(cache'.dv, sb).chain; // ensures
-          assert ChainFrom(cache'.dv, sb) == ChainFrom(cache.dv, sb);
-          if ChainFrom(cache'.dv, sb).chain.None? {
-            assert ChainFrom(cache'.dv, sb').chain.None?;
-          } else {
-	          calc {
-	            ChainFrom(cache'.dv, sb').chain.value.recs;
-	              {
-	                assert sb'.freshestCU.Some?;
-	                assert sb'.freshestCU.value in cache'.dv;
-	                assert parse(cache'.dv[sb'.freshestCU.value]).Some?;
-	                assert v'.marshalledLSN == v.unmarshalledLSN();
-	
-	                var cr := ChainFrom(cache'.dv, sb');
-	                assert cr.chain.Some?;
-	                var marshalledLsn := v'.marshalledLSN - 1;
-	                var idx := cr.chain.value.locate[marshalledLsn];
-	
-	                calc {
-	                  v'.FreshestMarshalledCU();
-	                  Some(v'.lsnToCU[v'.marshalledLSN-1]);
-	                  Some(CUForChainIdx(cr.chain.value, idx));
-	                  Some(newCU);
-	                }
-	                assert sb'.freshestCU == Some(newCU);
-	                assert sb'.boundaryLSN == v.boundaryLSN;
-	                assert sb' == Superblock(Some(newCU), v.boundaryLSN);
-	                assert MappingFor(cache, sb') == v'.lsnToCU;
-	                assert v'.lsnToCU[marshalledLsn] == CUForChainIdx(cr.chain.value, idx);
-	                assert v'.lsnToCU[marshalledLsn] == newCU;
-	                assert v'.lsnToCU[v'.marshalledLSN - 1] == newCU; // CorrectMapping isn't defined
-	                assert newCU == v'.FreshestMarshalledCU().value;
-	                assert sb'.freshestCU.value == newCU;
-	                assert jr == parse(cache'.dv[sb'.freshestCU.value]).value;  // CorrectMapping isn't defined.
-	                assert !(jr.messageSeq.seqEnd <= sb'.boundaryLSN);
-	                assert !(jr.messageSeq.seqStart <= sb.boundaryLSN);
-	                assert !(jr.priorCU.None?);
-	              }
-	            [jr] + ChainFrom(MapRemove1(cache'.dv, sb'.freshestCU.value), jr.priorSB(sb')).chain.value.recs;
-	            [jr] + ChainFrom(MapRemove1(cache'.dv, sb'.freshestCU.value), sb).chain.value.recs;
-	            [jr] + ChainFrom(cache.dv, sb).chain.value.recs;
-	              // Framing argument here
-	            [jr] + ChainFrom(cache.dv, sb).chain.value.recs;
-	          }
-	          calc {
-	            ChainAsMsgSeq(v', cache');
-	            ChainFrom(cache'.dv, sb').chain.value.interp.Concat(TailToMsgSeq(v'));
-	            new_chain_msgseq.Concat(new_tail_msgseq);
-	            new_chain_msgseq;
-	            orig_chain_msgseq.Concat(orig_tail_msgseq);
-	            ChainFrom(cache.dv, sb).chain.value.interp.Concat(TailToMsgSeq(v));
-	            ChainAsMsgSeq(v, cache);
-	          }
-	          assume false; // this is the slightly harder case, because the chain actually changes.
-	          assert ChainAsMsgSeq(v, cache) == ChainAsMsgSeq(v', cache');
+          assert CacheIfc.WritesApplied(cache, cache', cacheOps);
+          calc {
+            UnmarshalledMessageSeq(v, cache);
+            v.marshalledLookup.interp().Concat(TailToMsgSeq(v));
+              { UniqueChainLookup(cache, v.marshalledLookup, ChainFrom(cache, v.marshalledLookup.last().sb)); }  // Use invariant
+            ChainFrom(cache, v.marshalledLookup.last().sb).interp().Concat(TailToMsgSeq(v));
+            ChainFrom(cache', Superblock(Some(newCU), v.boundaryLSN)).interp();
+            ChainFrom(cache', Superblock(Some(newCU), v.boundaryLSN)).interp().Concat(TailToMsgSeq(v'));
+            v'.marshalledLookup.interp().Concat(TailToMsgSeq(v'));
+            UnmarshalledMessageSeq(v', cache');
           }
+
+//          assert ChainFrom(cache'.dv, v'.CurrentSuperblock()).chain.Some?;
+//          var sb := v.CurrentSuperblock();
+//          var sb' := v'.CurrentSuperblock();
+//          var orig_chain_msgseq := ChainFrom(cache.dv, sb).chain.value.interp;
+//          var orig_tail_msgseq := TailToMsgSeq(v);
+//          var new_chain_msgseq := ChainFrom(cache'.dv, sb').chain.value.interp;
+//          var new_tail_msgseq := TailToMsgSeq(v');
+//
+//          var priorCU := if v.marshalledLSN == v.boundaryLSN then None else Some(v.lsnToCU[v.marshalledLSN-1]);
+//          var jr := JournalRecord(TailToMsgSeq(v), priorCU);
+//          var sb_old := jr.priorSB(sb');
+//          assert sb_old == sb;
+//
+//          assert newCU !in IReads(cache, sb);
+//          assert DiskViewsEquivalentForSeq(cache.dv, cache'.dv, IReads(cache, sb));
+//          FrameOneChain(cache, cache', sb);
+////          assert ChainFrom(cache.dv, sb).chain == ChainFrom(cache'.dv, sb).chain; // ensures
+//          assert ChainFrom(cache'.dv, sb) == ChainFrom(cache.dv, sb);
+//          if ChainFrom(cache'.dv, sb).chain.None? {
+//            assert ChainFrom(cache'.dv, sb').chain.None?;
+//          } else {
+//	          calc {
+//	            ChainFrom(cache'.dv, sb').chain.value.recs;
+//	              {
+//	                assert sb'.freshestCU.Some?;
+//	                assert sb'.freshestCU.value in cache'.dv;
+//	                assert parse(cache'.dv[sb'.freshestCU.value]).Some?;
+//	                assert v'.marshalledLSN == v.unmarshalledLSN();
+//	
+//	                var cr := ChainFrom(cache'.dv, sb');
+//	                assert cr.chain.Some?;
+//	                var marshalledLsn := v'.marshalledLSN - 1;
+//	                var idx := cr.chain.value.locate[marshalledLsn];
+//	
+//	                calc {
+//	                  v'.FreshestMarshalledCU();
+//	                  Some(v'.lsnToCU[v'.marshalledLSN-1]);
+//	                  Some(CUForChainIdx(cr.chain.value, idx));
+//	                  Some(newCU);
+//	                }
+//	                assert sb'.freshestCU == Some(newCU);
+//	                assert sb'.boundaryLSN == v.boundaryLSN;
+//	                assert sb' == Superblock(Some(newCU), v.boundaryLSN);
+//	                assert MappingFor(cache, sb') == v'.lsnToCU;
+//	                assert v'.lsnToCU[marshalledLsn] == CUForChainIdx(cr.chain.value, idx);
+//	                assert v'.lsnToCU[marshalledLsn] == newCU;
+//	                assert v'.lsnToCU[v'.marshalledLSN - 1] == newCU; // CorrectMapping isn't defined
+//	                assert newCU == v'.FreshestMarshalledCU().value;
+//	                assert sb'.freshestCU.value == newCU;
+//	                assert jr == parse(cache'.dv[sb'.freshestCU.value]).value;  // CorrectMapping isn't defined.
+//	                assert !(jr.messageSeq.seqEnd <= sb'.boundaryLSN);
+//	                assert !(jr.messageSeq.seqStart <= sb.boundaryLSN);
+//	                assert !(jr.priorCU.None?);
+//	              }
+//	            [jr] + ChainFrom(MapRemove1(cache'.dv, sb'.freshestCU.value), jr.priorSB(sb')).chain.value.recs;
+//	            [jr] + ChainFrom(MapRemove1(cache'.dv, sb'.freshestCU.value), sb).chain.value.recs;
+//	            [jr] + ChainFrom(cache.dv, sb).chain.value.recs;
+//	              // Framing argument here
+//	            [jr] + ChainFrom(cache.dv, sb).chain.value.recs;
+//	          }
+//	          calc {
+//	            ChainAsMsgSeq(v', cache');
+//	            ChainFrom(cache'.dv, sb').chain.value.interp.Concat(TailToMsgSeq(v'));
+//	            new_chain_msgseq.Concat(new_tail_msgseq);
+//	            new_chain_msgseq;
+//	            orig_chain_msgseq.Concat(orig_tail_msgseq);
+//	            ChainFrom(cache.dv, sb).chain.value.interp.Concat(TailToMsgSeq(v));
+//	            ChainAsMsgSeq(v, cache);
+//	          }
+//	          assume false; // this is the slightly harder case, because the chain actually changes.
+//	          assert ChainAsMsgSeq(v, cache) == ChainAsMsgSeq(v', cache');
+//          }
         }
         case AdvanceCleanStep(newClean) => {
-          assert cacheOps == [];
-          CacheLemmasMod.EquivalentCaches(cache, cache', cacheOps);
-          assert ChainAsMsgSeq(v, cache) == ChainAsMsgSeq(v', cache');
+//          assert cacheOps == [];
+//          CacheLemmasMod.EquivalentCaches(cache, cache', cacheOps);
+//          assert ChainAsMsgSeq(v, cache) == ChainAsMsgSeq(v', cache');
         }
       }
-      assert ChainAsMsgSeq(v, cache) == ChainAsMsgSeq(v', cache');
+//      assert ChainAsMsgSeq(v, cache) == ChainAsMsgSeq(v', cache');
     }
     assert IM(v, cache, base) == IM(v', cache', base);
   }
